compiler/src/casper/types/MRStage.java
@@ -1,0 +1,14 @@
+package casper.types;
+
+import java.util.List;
+import java.util.Map;
+
+import casper.SketchParser.KvPair;
+
+public class MRStage {
+	public int stageType = -1;
+	public Map<String,List<KvPair>> mapEmits = null;
+	public Map<String,String> reduceExps = null;
+	public Map<String,String> initExps = null;
+	public Map<String,String> mergeExps = null;
+}
