bin/templates/dafny_skeleton.dfy
@@ -7,36 +7,18 @@ include "utils.dfy"
 /***************************** DO MAP ***************************************/
 
 <emit-funcs>
-function domap (<mapper-args-decl>) : <domap-emit-type>
-    <emit-requires>
-    ensures domap(<mapper-args-call>) == <domap-emits>
-{
-    <domap-emits>
-}
+
+<do-map-functions>
 
 /***************************** MAPPER ***************************************/
 
-function mapper (<mapper-args-decl>) : <domap-emit-type>
-    <mapper-requires>
-{
-    if <terminate-condition> then []
-    else domap(<mapper-args-call-inductive>) + mapper(<mapper-args-call-inductive>)
-}
+<mapper-functions>
 
 /***************************** DO REDUCE ************************************/
+
 <reduce-functions>
 
-function doreduce(input: <domap-emit-type>, casper_key: <doreduce-key-type><reducer-args-decl>) : <output-type>
-    <key-requires>
-    ensures (|input| > 0 && input[0].0 == casper_key) ==> 
-        doreduce(input, casper_key<reducer-args-call>) == (<reduce-exp>)
-    ensures (|input| > 0 && input[0].0 != casper_key) ==> 
-        doreduce(input, casper_key<reducer-args-call>) == doreduce(input[1..], casper_key<reducer-args-call>)
-{
-    if input == [] then (<reduce-init-value> )
-    else if input[0].0 == casper_key then (<reduce-exp>)
-    else doreduce(input[1..], casper_key<reducer-args-call>)
-}
+<do-reduce-functions>
 
 /******************************* HARNESS ************************************/    
 
