bin/output/main_double_0.dfy
@@ -1,0 +1,78 @@
+/***************************** INCLUDES *************************************/
+include "utils.dfy"
+
+/******************************* UDTS ***************************************/
+class MulVecSca{
+}
+
+
+/***************************** DO MAP ***************************************/
+
+function emit_0_0(a: seq<int>, i0: int, i: int, loop0: bool, b: int) : <domap-emit-type>
+	<emit-requires>
+	ensures emit_0_0(a, i0, i, loop0, b) == [((1,i),(b*a[i],b))]
+{
+	[((1,i),(b*a[i],b))]
+}
+
+
+
+function domap_0 (a: seq<int>, i0: int, i: int, loop0: bool, b: int) : <domap-emit-type>
+    <emit-requires>
+    ensures domap_0(a, i0, i, loop0, b) == emit_0_0(a, i0, i, loop0, b)
+{
+    emit_0_0(a, i0, i, loop0, b)
+}
+
+/***************************** MAPPER ***************************************/
+
+function mapper_0 (a: seq<int>, i0: int, i: int, loop0: bool, b: int) : <domap-emit-type>
+    <mapper-requires>
+{
+    if <terminate-condition> then []
+    else domap_0(a, i0, i-1, loop0, b) + mapper_0(a, i0, i-1, loop0, b)
+}
+
+/***************************** DO REDUCE ************************************/
+
+
+
+
+
+/******************************* HARNESS ************************************/    
+
+predicate loopInvariant (a: seq<int>, temp: seq<int>, temp0: seq<int>, i: int, i0: int, loop0: bool, b: int)
+    requires  |temp| == |temp0|
+	
+{
+    0 <= i <= |a| &&
+	(forall k :: 0 <= k < |temp| ==> temp[k] == (mapper_0(,loop0,b,temp0))[k])	
+}
+
+predicate postCondition (a: seq<int>, temp: seq<int>, temp0: seq<int>, i: int, i0: int, loop0: bool, b: int)
+    requires  |temp| == |temp0|
+	
+{
+    i == |a| &&
+	(forall k :: 0 <= k < |temp| ==> temp[k] == (mapper_0(,loop0,b,temp0))[k])	
+}
+
+method harness (a: seq<int>, temp: seq<int>, temp0: seq<int>, b: int, i: int)
+    requires  |temp| == |temp0|
+	requires  forall k :: 0 <= k < |temp0| ==> temp0[k] == 0
+{
+    var loop0 := false;
+	var i0 := 0;
+	
+    assert loopInvariant(a,temp0,temp0,i0,i0,loop0,b);
+
+	if(loopInvariant(a,temp,temp0,i,i0,loop0,b) && (i<|a|))
+	{
+		assert loopInvariant(a,int_setter(temp,i,(int_getter(a,i)*b)),temp0,(i+1),i0,loop0,b);
+	}
+
+	if(loopInvariant(a,temp,temp0,i,i0,loop0,b) && !(i<|a|))
+	{
+		assert postCondition(a,temp,temp0,i,0,loop0,b);
+	}
+}
