bin/output/main_int_0.dfy
@@ -1,0 +1,68 @@
+/***************************** INCLUDES *************************************/
+include "utils.dfy"
+
+/******************************* UDTS ***************************************/
+class Count{
+}
+
+
+/***************************** DO MAP ***************************************/
+
+
+
+
+
+/***************************** MAPPER ***************************************/
+
+
+
+/***************************** DO REDUCE ************************************/
+
+function reduce_0_count(val1: int, val2: int, loop0: bool, count0: int) : int
+{
+	(1+val1)
+}
+
+
+function doreduce_0(data: seq<int>, i: int, loop0: bool, count0: int) : int
+    requires 0 <= i <= |data|
+{
+    if i == 0 then 0
+    else (reduce_0_count(doreduce_0(data,i-1,loop0,count0),data[i-1],loop0,count0))
+}
+
+/******************************* HARNESS ************************************/    
+
+predicate loopInvariant (data: seq<int>, count: int, count0: int, i: int, i0: int, loop0: bool)
+    
+{
+    0 <= i <= |data| &&
+	(count == (doreduce_0(data,i,loop0,count0)))
+}
+
+predicate postCondition (data: seq<int>, count: int, count0: int, i: int, i0: int, loop0: bool)
+    
+{
+    i == |data| &&
+	(count == (doreduce_0(data,i,loop0,count0)))
+}
+
+method harness (data: seq<int>, count: int, i: int)
+    
+{
+    var count0 := 0;
+	var loop0 := false;
+	var i0 := 0;
+	
+    assert loopInvariant(data,count0,count0,i0,i0,loop0);
+
+	if(loopInvariant(data,count,count0,i,i0,loop0) && (i<|data|))
+	{
+		assert loopInvariant(data,(count+1),count0,(i+1),i0,loop0);
+	}
+
+	if(loopInvariant(data,count,count0,i,i0,loop0) && !(i<|data|))
+	{
+		assert postCondition(data,count,0,i,0,loop0);
+	}
+}
